wip, elaboration

examples/dsls/mini_steel/MiniSteel.fst
@@ -18,8 +18,11 @@ type term =
   | Tm_Var      : v:var -> term
   | Tm_FVar     : l:lident -> term
   | Tm_Constant : c:constant -> term
+  | Tm_Abs      : t:typ -> body:term -> term
   | Tm_PureApp  : head:term -> arg:term -> term
   | Tm_Let      : t:typ -> e1:term -> e2:term -> term  
+  | Tm_STApp    : head:term -> arg:term -> term  
+  | Tm_Bind     : t:typ -> e1:term -> e2:term -> term
   | Tm_Emp      : term
   | Tm_Pure     : p:term -> term
   | Tm_Star     : l:term -> r:term -> term
@@ -28,8 +31,6 @@ type term =
   | Tm_Arrow    : t:typ -> body:comp -> term 
   | Tm_Type     : term
   | Tm_VProp    : term
-  | Tm_STApp    : head:term -> arg:term -> term  
-  | Tm_Bind     : t:typ -> e1:term -> e2:term -> term
   | Tm_If       : b:term -> then_:term -> else_:term -> term
 
 and comp = 
@@ -83,11 +84,60 @@ let eqn = term & term
 let binding = either typ eqn
 let env = list (var & binding)
 
-assume
-val elab_term (t:term) : R.term
+let tun = R.pack_ln R.Tv_Unknown
 
 assume
-val elab_comp (c:comp) : R.comp
+val mk_st (res pre post:R.term) : R.comp
+
+let rec elab_term (t:term)
+  : R.term
+  = let open R in
+    match t with
+    | Tm_BVar n -> 
+      let bv = pack_bv (RT.make_bv n tun) in
+      pack_ln (Tv_BVar bv)
+      
+    | Tm_Var n ->
+      // tun because type does not matter at a use site
+      let bv = pack_bv (RT.make_bv n tun) in
+      pack_ln (Tv_Var bv)
+
+    | Tm_FVar l ->
+      pack_ln (Tv_FVar (pack_fv l))
+
+    | Tm_Abs t b ->
+      let t = elab_term t in
+      let b = elab_term b in
+      R.pack_ln (Tv_Abs (RT.as_binder 0 t) b)
+      
+    | Tm_PureApp e1 e2 ->
+      let e1 = elab_term e1 in
+      let e2 = elab_term e2 in
+      pack_ln (Tv_App e1 (e2, Q_Explicit))
+
+    | Tm_Arrow t c ->
+      let t = elab_term t in
+      let c = elab_comp c in
+      R.pack_ln 
+        (R.Tv_Arrow 
+          (RT.as_binder 0 t) 
+          c)
+
+    | _ -> admit()
+
+and elab_comp (c:comp) 
+  : R.comp
+  = match c with
+    | C_Tot t ->
+      let t = elab_term t in 
+      RT.mk_total t
+
+    | C_ST c ->
+      let res = elab_term c.res in
+      let pre = elab_term c.pre in
+      let post = elab_term c.post in
+      mk_st res pre post
+
 
 assume
 val extend_env_l (f:fstar_top_env) (g:env) : fstar_env
@@ -131,6 +181,25 @@ type bind_comp (f:fstar_top_env) : env -> st_comp -> var -> st_comp -> st_comp -
         ~(x `Set.mem` freevars c2.res) 
       } ->
       bind_comp f g c1 x c2 ({res = c2.res; pre = c1.pre; post=c2.post})
+
+
+
+assume
+val tm_bool : term
+assume
+val tm_true : term
+assume
+val tm_false : term
+let mk_eq2 t (e0 e1:term) 
+  : term
+  = Tm_PureApp
+         (Tm_PureApp (Tm_PureApp (Tm_FVar R.eq2_qn) t)
+                      e0) e1
+
+let return_comp (t:typ) (e:term) =
+  { res = t;
+    pre = Tm_Emp;
+    post = Tm_Pure (mk_eq2 t (Tm_BVar 0) e) }
 
 
 [@@erasable]
@@ -191,7 +260,7 @@ type vprop_equiv (f:fstar_top_env) : env -> term -> term -> Type =
      ty:typ ->
      t0:term ->
      t1:term ->
-     vprop_equiv f g (open_term t0 x) (open_term t1 x) ->
+     vprop_equiv f ((x, Inl ty)::g) (open_term t0 x) (open_term t1 x) ->
      vprop_equiv f g (Tm_ExistsSL ty t0) (Tm_ExistsSL ty t1)
 
   | VE_Fa:
@@ -200,9 +269,8 @@ type vprop_equiv (f:fstar_top_env) : env -> term -> term -> Type =
      ty:typ ->
      t0:term ->
      t1:term ->
-     vprop_equiv f g (open_term t0 x) (open_term t1 x) ->
+     vprop_equiv f ((x, Inl ty)::g) (open_term t0 x) (open_term t1 x) ->
      vprop_equiv f g (Tm_ForallSL ty t0) (Tm_ForallSL ty t1)
-
 
 [@@erasable]
 noeq
@@ -215,23 +283,6 @@ type st_equiv (f:fstar_top_env) : env -> st_comp -> st_comp -> Type =
       vprop_equiv f g c1.pre c2.pre ->
       vprop_equiv f ((x, Inl c1.res)::g) (open_term c1.post x) (open_term c2.post x) ->      
       st_equiv f g c1 c2
-
-assume
-val tm_bool : term
-assume
-val tm_true : term
-assume
-val tm_false : term
-let mk_eq2 t (e0 e1:term) 
-  : term
-  = Tm_PureApp
-         (Tm_PureApp (Tm_PureApp (Tm_FVar R.eq2_qn) t)
-                      e0) e1
-
-let return_comp (t:typ) (e:term) =
-  { res = t;
-    pre = Tm_Emp;
-    post = Tm_Pure (mk_eq2 t (Tm_BVar 0) e) }
 
 [@@erasable]
 noeq
@@ -310,6 +361,57 @@ and tot_typing (f:fstar_top_env) (g:env) (e:term) (t:typ) =
 and st_typing (f:fstar_top_env) (g:env) (e:term) (st:st_comp) = 
   src_typing f g e (C_ST st)
 
+let star_typing_inversion (f:_) (g:_) (t0 t1:term) (d:tot_typing f g (Tm_Star t0 t1) Tm_VProp)
+  : (tot_typing f g t0 Tm_VProp &
+     tot_typing f g t1 Tm_VProp)
+  = admit()
+
+let star_typing (#f:_) (#g:_) (#t0 #t1:term)
+                (d0:tot_typing f g t0 Tm_VProp)
+                (d1:tot_typing f g t1 Tm_VProp)
+  : tot_typing f g (Tm_Star t0 t1) Tm_VProp
+  = admit()
+
+
+let emp_typing (#f:_) (#g:_) 
+  : tot_typing f g Tm_Emp Tm_VProp
+  = admit()
+
+let rec vprop_equiv_typing (f:_) (g:_) (t0 t1:term) (v:vprop_equiv f g t0 t1)
+  : GTot ((tot_typing f g t0 Tm_VProp -> tot_typing f g t1 Tm_VProp) &
+          (tot_typing f g t1 Tm_VProp -> tot_typing f g t0 Tm_VProp))
+         (decreases v)
+  = match v with
+    | VE_Refl _ _ -> (fun x -> x), (fun x -> x)
+    | VE_Sym _ _ _ v' -> 
+      let f, g = vprop_equiv_typing f g t1 t0 v' in
+      g, f
+    | VE_Trans g t0 t2 t1 v02 v21 ->
+      let f02, f20 = vprop_equiv_typing _ _ _ _ v02 in
+      let f21, f12 = vprop_equiv_typing _ _ _ _ v21 in
+      (fun x -> f21 (f02 x)), 
+      (fun x -> f20 (f12 x))
+    | VE_Ctxt g s0 s1 s0' s1' v0 v1 ->
+      let f0, f0' = vprop_equiv_typing _ _ _ _ v0 in
+      let f1, f1' = vprop_equiv_typing _ _ _ _ v1 in      
+      let ff (x:tot_typing f g (Tm_Star s0 s1) Tm_VProp)
+        : tot_typing f g (Tm_Star s0' s1') Tm_VProp
+        = let s0_typing, s1_typing = star_typing_inversion _ _ _ _ x in
+          let s0'_typing, s1'_typing = f0 s0_typing, f1 s1_typing in
+          star_typing s0'_typing s1'_typing
+      in
+      let gg (x:tot_typing f g (Tm_Star s0' s1') Tm_VProp)
+        : tot_typing f g (Tm_Star s0 s1) Tm_VProp
+        = let s0'_typing, s1'_typing = star_typing_inversion _ _ _ _ x in
+          star_typing (f0' s0'_typing) (f1' s1'_typing)        
+      in
+      ff, gg
+
+
+    | _ -> admit()
+      
+
+  
 module L = FStar.List.Tot
 let max (n1 n2:nat) = if n1 < n2 then n2 else n1
 
@@ -555,7 +657,11 @@ let split_vprop (f:fstar_top_env)
                                ctxt =
          VE_Trans _ _ _ _ d (VE_Sym _ _ _ (vprop_list_equiv f g ctxt))
        in
-       let typing : tot_typing f g (list_as_vprop frame) Tm_VProp = magic () in
+       let typing : tot_typing f g (list_as_vprop frame) Tm_VProp = 
+         let fwd, bk = vprop_equiv_typing _ _ _ _ d in
+         let star_typing = bk ctxt_typing in
+         snd (star_typing_inversion _ _ _ _ star_typing)
+       in
        (| list_as_vprop frame, typing, d |)
 
 let try_frame_pre (#f:fstar_top_env)
@@ -651,6 +757,10 @@ let rec check (f:fstar_top_env)
           (| _, T_Bind _ _ _ _ _ _ _ d1 d2 b |)
      )
 
+    | Tm_Abs _ _
     | Tm_If _ _ _ ->
-      T.fail "Not handling if yet"
+      T.fail "Not handling if/abs yet"
 
+////////////////////////////////////////////////////////////////////////////////
+// elaboration
+////////////////////////////////////////////////////////////////////////////////
